feat: Formal Verification for updated circuits (#1644)
* bump lean version

* update circuits with input hashing

* checkpoint on rangetrees

* no indices

* remove next index

* progress on address tree

* extract all circuits

* checkpoint

* bring back some tests

* catch-up old mains

* batch append circuit

* add proofs for BatchUpdate

* soundness and completeness for address append

* clean up sorries

* state main props for address append

* fix change

* fix tags

* correct tree depths

prover/server/formal-verification/Main.lean
@@ -5,42 +5,252 @@ import FormalVerification.Merkle
 
 open LightProver (F)
 
+open LightProver renaming InclusionCircuit_10_10_10_32_10_10_32 → InclusionCircuit,
+                          NonInclusionCircuit_10_10_10_10_10_40_10_10_40 → NonInclusionCircuit,
+                          CombinedCircuit_10_10_10_32_10_10_10_10_10_10_40_10 → CombinedCircuit,
+                          BatchAppendWithProofsCircuit_10_10_32_10_32_10 → BatchAppendWithProofsCircuit,
+                          BatchUpdateCircuit_10_10_10_32_10_10_32_10 → BatchUpdateCircuit,
+                          BatchAddressTreeAppendCircuit_10_10_10_40_10_10_40_10_10_40 → BatchAddressTreeAppendCircuit
+
+abbrev SD := 32
+abbrev AD := 40
+abbrev B := 10
+
 theorem poseidon₂_testVector :
-  poseidon₂ vec![1, 2] = 7853200120776062878684798364095072458815029376092732009249414926327459813530 := rfl
+  poseidon₂ vec![1, 2] = 7853200120776062878684798364095072458815029376092732009249414926327459813530 := by native_decide
 
 theorem poseidon₃_testVector :
-  poseidon₃ vec![1, 2, 3] = 6542985608222806190361240322586112750744169038454362455181422643027100751666 := rfl
+  poseidon₃ vec![1, 2, 3] = 6542985608222806190361240322586112750744169038454362455181422643027100751666 := by native_decide
 
-theorem InclusionCircuit.correct
-  [Fact (CollisionResistant poseidon₂)]
-  {trees : Vector (MerkleTree F poseidon₂ 26) 8}
-  {leaves : Vector F 8}:
-    (∃p₁ p₂, LightProver.InclusionCircuit_8_8_8_26_8_8_26 (trees.map (·.root)) leaves p₁ p₂)
-    ↔ ∀i (_: i∈[0:8]), leaves[i] ∈ trees[i]
-  := InclusionCircuit_correct
+axiom poseidon₂_collisionResistant : CollisionResistant poseidon₂
+instance : Fact (CollisionResistant poseidon₂) := ⟨poseidon₂_collisionResistant⟩
 
-theorem NonInclusionCircuit.correct
-  [Fact (CollisionResistant poseidon₃)]
-  [Fact (CollisionResistant poseidon₂)]
-  {trees : Vector (RangeTree 26) 8}
-  {leaves : Vector F 8}:
-    (∃p₁ p₂ p₃ p₄ p₅,
-      LightProver.NonInclusionCircuit_8_8_8_8_8_8_26_8_8_26 (trees.map (·.val.root)) leaves p₁ p₂ p₃ p₄ p₅)
-    ↔ ∀i (_: i∈[0:8]), leaves[i] ∈ trees[i]
-  := NonInclusionCircuit_correct
+axiom poseidon₃_collisionResistant : CollisionResistant poseidon₃
+instance : Fact (CollisionResistant poseidon₃) := ⟨poseidon₃_collisionResistant⟩
 
-theorem CombinedCircuit.correct
-  [Fact (CollisionResistant poseidon₃)]
-  [Fact (CollisionResistant poseidon₂)]
-  {inclusionTrees : Vector (MerkleTree F poseidon₂ 26) 8}
-  {nonInclusionTrees : Vector (RangeTree 26) 8}
-  {inclusionLeaves nonInclusionLeaves : Vector F 8}:
-    (∃p₁ p₂ p₃ p₄ p₅ p₆ p₇,
-      LightProver.CombinedCircuit_8_8_8_26_8_8_8_8_8_8_8_26_8
+axiom poseidon₂_nez : poseidon₂_no_zero_preimage
+instance : Fact poseidon₂_no_zero_preimage := ⟨poseidon₂_nez⟩
+
+namespace InclusionCircuit
+
+theorem sound_and_complete
+  {trees : List.Vector (MerkleTree F poseidon₂ SD) B}
+  {leaves : List.Vector F B}:
+    (∃ih p₁ p₂, InclusionCircuit ih (trees.map (·.root)) leaves p₁ p₂)
+    ↔ ∀i (_: i∈[0:B]), leaves[i] ∈ trees[i]
+  := by simp [InclusionCircuit_correct]
+
+theorem inputHash_deterministic:
+    InclusionCircuit h₁ trees leaves i₁ p₁ ∧
+    InclusionCircuit h₂ trees leaves i₂ p₂ →
+    h₁ = h₂ := by
+  simp only [InclusionCircuit_rw]
+  intros
+  simp_all
+
+theorem inputHash_injective:
+    InclusionCircuit h trees₁ leaves₁ i₁ p₁ →
+    InclusionCircuit h trees₂ leaves₂ i₂ p₂ →
+    trees₁ = trees₂ ∧ leaves₁ = leaves₂ := by
+  simp only [InclusionCircuit_rw]
+  rintro ⟨h₁, _⟩ ⟨h₂, _⟩
+  cases h₁
+  exact inputHash_correct.mp h₂
+
+end InclusionCircuit
+
+namespace NonInclusionCircuit
+
+theorem sound_and_complete
+  {trees : List.Vector (RangeVector (2^AD)) B}
+  {leaves : List.Vector F B}:
+    (∃ih p₁ p₂ p₃ p₄,
+      NonInclusionCircuit ih (trees.map (·.root)) leaves p₁ p₂ p₃ p₄)
+    ↔ ∀i (_: i∈[0:B]), leaves[i].val ∈ trees[i]
+  := by
+    conv => lhs; arg 1; intro ih; rw [NonInclusionCircuit_correct]
+    simp
+
+theorem inputHash_deterministic:
+    NonInclusionCircuit h₁ trees leaves lo₁ hi₁ i₁ p₁ →
+    NonInclusionCircuit h₂ trees leaves lo₂ hi₂ i₂ p₂ →
+    h₁ = h₂ := by
+  unfold NonInclusionCircuit
+  simp_all [TwoInputsHashChain_rw, LightProver.Gates, GatesGnark8]
+
+theorem inputHash_injective:
+    NonInclusionCircuit h trees₁ leaves₁ lo₁ hi₁ i₁ p₁ →
+    NonInclusionCircuit h trees₂ leaves₂ lo₂ hi₂ i₂ p₂ →
+    trees₁ = trees₂ ∧ leaves₁ = leaves₂ := by
+  unfold NonInclusionCircuit
+  simp only [TwoInputsHashChain_rw, LightProver.Gates, GatesGnark8]
+  rintro ⟨h₁, _⟩ ⟨h₂, _⟩
+  cases h₁
+  exact inputHash_correct.mp h₂
+
+end NonInclusionCircuit
+
+namespace CombinedCircuit
+
+theorem sound_and_complete
+  {inclusionTrees : List.Vector (MerkleTree F poseidon₂ SD) B}
+  {nonInclusionTrees : List.Vector (RangeVector (2^AD)) B}
+  {inclusionLeaves nonInclusionLeaves : List.Vector F B}:
+    (∃ih p₁ p₂ p₃ p₄ p₅ p₆,
+      CombinedCircuit
+        ih
         (inclusionTrees.map (·.root)) inclusionLeaves p₁ p₂
-        (nonInclusionTrees.map (·.val.root)) nonInclusionLeaves p₃ p₄ p₅ p₆ p₇)
-    ↔ ∀i (_: i∈[0:8]), inclusionLeaves[i] ∈ inclusionTrees[i]
-                      ∧ nonInclusionLeaves[i] ∈ nonInclusionTrees[i]
-  := CombinedCircuit_correct
+        (nonInclusionTrees.map (·.root)) nonInclusionLeaves p₃ p₄ p₅ p₆)
+    ↔ ∀i (_: i∈[0:B]), inclusionLeaves[i] ∈ inclusionTrees[i]
+                      ∧ nonInclusionLeaves[i].val ∈ nonInclusionTrees[i]
+  := by
+    conv => lhs; arg 1; intro ih; rw [CombinedCircuit_correct]
+    simp
+
+theorem inputHash_deterministic:
+    CombinedCircuit h₁ inclusionTrees inclusionLeaves p₁ p₂ nonInclusionTrees nonInclusionLeaves p₃ p₄ p₅ p₆ →
+    CombinedCircuit h₂ inclusionTrees inclusionLeaves q₁ q₂ nonInclusionTrees nonInclusionLeaves q₃ q₄ q₅ q₆ →
+    h₁ = h₂ := by
+  unfold CombinedCircuit
+  simp_all [TwoInputsHashChain_rw, LightProver.Gates, GatesGnark8]
+
+theorem inputHash_injective:
+    CombinedCircuit h inclusionTrees₁ inclusionLeaves₁ p₁ p₂ nonInclusionTrees₁ nonInclusionLeaves₁ p₃ p₄ p₅ p₆ →
+    CombinedCircuit h inclusionTrees₂ inclusionLeaves₂ q₁ q₂ nonInclusionTrees₂ nonInclusionLeaves₂ q₃ q₄ q₅ q₆ →
+    inclusionTrees₁ = inclusionTrees₂ ∧ inclusionLeaves₁ = inclusionLeaves₂ ∧ nonInclusionTrees₁ = nonInclusionTrees₂ ∧ nonInclusionLeaves₁ = nonInclusionLeaves₂ := by
+  unfold CombinedCircuit
+  simp only [TwoInputsHashChain_rw, Poseidon2_iff_uniqueAssignment, LightProver.Gates, GatesGnark8, GatesDef.eq]
+  rintro ⟨h₁, _⟩ ⟨h₂, _⟩
+  rw [h₁] at h₂
+  simp only [CollisionResistant_def, List.Vector.eq_cons, inputHash_correct] at h₂
+  simp_all
+
+end CombinedCircuit
+
+namespace BatchAppendWithProofsCircuit
+
+theorem sound_and_complete
+  {tree : MerkleTree F poseidon₂ SD} {newRoot startIndex : F} {leaves : List.Vector F B}:
+    (∃ih oldLeaves merkleProofs lh,
+      BatchAppendWithProofsCircuit
+        ih tree.root newRoot lh startIndex oldLeaves leaves merkleProofs)
+    ↔
+    (startIndex.val + (B - 1) < 2^SD) ∧
+    ∃(newTree : MerkleTree F poseidon₂ SD), newRoot = newTree.root ∧
+    ∀(i : Fin (2^SD)),
+      (i.val ∈ [startIndex.val:(startIndex.val + B)] → newTree[i] = if tree[i] = 0 then leaves[i.val - startIndex.val]! else tree[i]) ∧
+      (i.val ∉ [startIndex.val:(startIndex.val + B)] → newTree[i] = tree[i])
+  := by
+  simp [AppendWithProofs_rw]
+  rw [eq_comm, Option.map_eq_some']
+  simp [treeAppends_sound_and_complete]
+  apply Iff.intro
+  · tauto
+  · rintro ⟨_, t, _⟩
+    use t
+    tauto
+
+theorem inputHash_deterministic:
+    BatchAppendWithProofsCircuit h₁ oldRoot newRoot p₁ startIndex p₂ leaves p₃ ∧
+    BatchAppendWithProofsCircuit h₂ oldRoot newRoot q₁ startIndex q₂ leaves q₃ →
+    h₁ = h₂ := by
+  intro ⟨hp₁, hp₂⟩
+  have := (AppendWithProofs_rw1.mp (Exists.intro _ hp₁)).1
+  have := (AppendWithProofs_rw1.mp (Exists.intro _ hp₂)).1
+  simp_all
+
+theorem inputHash_injective:
+    BatchAppendWithProofsCircuit h oldRoot₁ newRoot₁ p₁ startIndex₁ p₂ leaves₁ p₃ ∧
+    BatchAppendWithProofsCircuit h oldRoot₂ newRoot₂ q₁ startIndex₂ q₂ leaves₂ q₃ →
+    oldRoot₁ = oldRoot₂ ∧ newRoot₁ = newRoot₂ ∧ startIndex₁ = startIndex₂ ∧ leaves₁ = leaves₂ := by
+  intro ⟨hp₁, hp₂⟩
+  have := (AppendWithProofs_rw1.mp (Exists.intro _ hp₁)).1
+  have := (AppendWithProofs_rw1.mp (Exists.intro _ hp₂)).1
+  simp_all [hashChain_injective, List.Vector.eq_cons]
+
+end BatchAppendWithProofsCircuit
+
+namespace BatchUpdateCircuit
+
+theorem sound_and_complete
+  {tree : MerkleTree F poseidon₂ SD} {newRoot : F} {leaves txHashes indices : List.Vector F B} (indices_distinct: ∀(i j : Fin B), i ≠ j → indices[i] ≠ indices[j]):
+  (∃ih ps ols lhh, BatchUpdateCircuit ih tree.root newRoot lhh txHashes leaves ols ps indices) ↔
+    ∃(newTree : MerkleTree F poseidon₂ SD), newRoot = newTree.root ∧
+    ∃(hr : ∀ (i:Fin B), indices[i].val < 2^SD),
+    (∀i: Fin B, newTree[indices[i].val]'(hr i) = poseidon₃ vec![leaves[i], indices[i], txHashes[i]]) ∧
+    (∀i: Fin (2^SD), ↑i.val ∉ indices → newTree[i] = tree[i]) := by
+  simp [BatchUpdateCircuit_rw1, batchUpdate_rec_rw, batchUpdates_sem_of_distinct indices_distinct]
+  apply Iff.intro <;> {
+    rintro ⟨nt, _⟩
+    use nt
+    simp_all
+  }
+
+theorem inputHash_deterministic :
+    BatchUpdateCircuit h₁ oldRoot newRoot lhh₁ txHashes leaves ols₁ ps₁ indices ∧
+    BatchUpdateCircuit h₂ oldRoot newRoot lhh₂ txHashes leaves ols₂ ps₂ indices →
+    h₁ = h₂ := by
+  intro ⟨hp₁, hp₂⟩
+  have := (BatchUpdateCircuit_rw1.mp (Exists.intro _ hp₁)).1
+  have := (BatchUpdateCircuit_rw1.mp (Exists.intro _ hp₂)).1
+  simp_all
+
+theorem inputHash_injective :
+    BatchUpdateCircuit h oldRoot₁ newRoot₁ lhh₁ txHashes₁ leaves₁ ols₁ ps₁ indices₁ ∧
+    BatchUpdateCircuit h oldRoot₂ newRoot₂ lhh₂ txHashes₂ leaves₂ ols₂ ps₂ indices₂ →
+    oldRoot₁ = oldRoot₂ ∧ newRoot₁ = newRoot₂ ∧ txHashes₁ = txHashes₂ ∧ leaves₁ = leaves₂ ∧ indices₁ = indices₂ := by
+  intro ⟨hp₁, hp₂⟩
+  have t₁ := (BatchUpdateCircuit_rw1.mp (Exists.intro _ hp₁)).1
+  have := (BatchUpdateCircuit_rw1.mp (Exists.intro _ hp₂)).1
+  rw [t₁] at this
+  simp_all [hashChain_injective, hashChain3_injective, List.Vector.eq_cons]
+
+end BatchUpdateCircuit
+
+namespace BatchAddressAppendTreeCircuit
+
+theorem sound {ranges : RangeVector (2^AD)} {elements : List.Vector F B} {newRoot : F}:
+    (∃pih hch si lev lenv lei lep nep, BatchAddressTreeAppendCircuit pih ranges.root newRoot hch si lev lenv lei lep elements nep) →
+    ∃newRanges : RangeVector (2^AD), newRanges.root = newRoot ∧ (∀i ∈ elements, i.val ∉ newRanges) ∧ (∀i, ↑i ∉ elements → (i ∈ ranges ↔ i ∈ newRanges)) := by
+  exact BatchAdressAppend_sound
+
+theorem complete {rv : RangeVector (2^AD)} {elements startIndex}
+    (startIndex_small : startIndex + B < 2^AD)
+    (elements_distinct : ∀(i j : Fin B), i ≠ j → elements[i] ≠ elements[j])
+    (elements_mem : ∀ i ∈ elements, i.val ∈ rv)
+    (indices_empty : ∀ i ∈ [startIndex:(startIndex + B)], rv.ranges i = none):
+    ∃lev lenv lei lep nep newRoot hch pih, BatchAddressTreeAppendCircuit pih rv.root newRoot hch startIndex lev lenv lei lep elements nep := by
+  apply BatchAddressAppend_complete <;> simp_all [getElem]
+  intro i hi
+  have := indices_empty i hi
+  simp [←this]
+  congr
+  rw [Nat.mod_eq_of_lt]
+  linarith [hi.2]
+
+theorem inputHash_deterministic:
+    BatchAddressTreeAppendCircuit h₁ oldRoot newRoot lhh₁ startIndex lev₁ lenv₁ lei₁ lep₁ elements nep₁ ∧
+    BatchAddressTreeAppendCircuit h₂ oldRoot newRoot lhh₂ startIndex lev₂ lenv₂ lei₂ lep₂ elements nep₂ →
+    h₁ = h₂ := by
+  intro ⟨hp₁, hp₂⟩
+  have h₁ := BatchAddressLoop_skip_tree (BatchAddressLoop_rw1.mp hp₁)
+  have h₂ := BatchAddressLoop_skip_tree (BatchAddressLoop_rw1.mp hp₂)
+  simp [HashChain_B_rw, LightProver.Gates, GatesGnark8, HashChain_4_rw] at h₁ h₂
+  simp_all
+
+theorem inputHash_injective:
+    BatchAddressTreeAppendCircuit h oldRoot₁ newRoot₁ lhh₁ startIndex₁ lev₁ lenv₁ lei₁ lep₁ elements₁ nep₁ ∧
+    BatchAddressTreeAppendCircuit h oldRoot₂ newRoot₂ lhh₂ startIndex₂ lev₂ lenv₂ lei₂ lep₂ elements₂ nep₂ →
+    oldRoot₁ = oldRoot₂ ∧ newRoot₁ = newRoot₂ ∧ startIndex₁ = startIndex₂ ∧ elements₁ = elements₂ := by
+  intro ⟨hp₁, hp₂⟩
+  have h₁ := BatchAddressLoop_skip_tree (BatchAddressLoop_rw1.mp hp₁)
+  have h₂ := BatchAddressLoop_skip_tree (BatchAddressLoop_rw1.mp hp₂)
+  simp [HashChain_B_rw, LightProver.Gates, GatesGnark8, HashChain_4_rw, hashChain_injective] at h₁ h₂
+  rcases h₁ with ⟨rfl, h₁⟩
+  rcases h₂ with ⟨rfl, h₂⟩
+  rw [h₁] at h₂
+  simp_all [hashChain_injective, List.Vector.eq_cons]
+
+end BatchAddressAppendTreeCircuit
 
 def main : IO Unit := pure ()
